library/init/category/reader.lean
@@ -8,16 +8,8 @@ prelude
 import init.category.transformers init.category.id
 universes u v w
 
-class monad_reader (r : out_param (Type u)) (m : Type u → Type v) [monad m] :=
-(reader {} {α : Type u} : (r → α) → m α)
-(read {} : m r := reader id)
-(reader := λ α f, f <$> read)
-
-
-export monad_reader (read)
-
-def reader_t (r : Type u) (m : Type u → Type v) (α : Type u) : Type (max u v) :=
-r → m α
+structure reader_t (r : Type u) (m : Type u → Type v) (α : Type u) : Type (max u v) :=
+(run : r → m α)
 
 @[reducible] def reader (r : Type u) := reader_t r id
 
@@ -29,31 +21,41 @@ section
   variables {α β : Type u}
 
   protected def read : reader_t r m r :=
-  λ r, pure r
-
-  protected def run : r → reader_t r m α → m α :=
-  λ r x, x r
+  ⟨pure⟩
 
   protected def pure (a : α) : reader_t r m α :=
-  λ r, pure a
+  ⟨λ r, pure a⟩
 
   protected def bind (x : reader_t r m α) (f : α → reader_t r m β) : reader_t r m β :=
-  λ r, do a ← x r,
-          f a r
+  ⟨λ r, do a ← x.run r,
+           (f a).run r⟩
 
   instance : monad (reader_t r m) :=
   { pure := @reader_t.pure _ _ _, bind := @reader_t.bind _ _ _ }
 
   protected def lift (a : m α) : reader_t r m α :=
-  λ r, a
+  ⟨λ r, a⟩
 
   instance (m) [monad m] : has_monad_lift m (reader_t r m) :=
   ⟨@reader_t.lift r m _⟩
+
+  protected def map {r m m'} [monad m] [monad m'] {α} (f : Π {α}, m α → m' α) : reader_t r m α → reader_t r m' α :=
+  λ x, ⟨λ r, f (x.run r)⟩
+
+  instance (r m m') [monad m] [monad m'] : monad_functor m m' (reader_t r m) (reader_t r m') :=
+  ⟨@reader_t.map r m m' _ _⟩
 end
 end reader_t
 
-def with_reader_t {r r' m} [monad m] {α} (f : r' → r) : reader_t r m α → reader_t r' m α :=
-λ x r, x (f r)
+class monad_reader_lift (r : out_param (Type u)) (m : out_param (Type u → Type v)) (n : Type u → Type w) :=
+[has_lift : has_monad_lift_t (reader_t r m) n]
+
+attribute [instance] monad_reader_lift.mk
+local attribute [instance] monad_reader_lift.has_lift
+
+def monad_reader_lift.read {r : Type u} {m : Type u → Type v} {n : Type u → Type w} [monad m] [monad_reader_lift r m n] : n r :=
+@monad_lift _ _ _ _ (reader_t.read : reader_t r m _)
+export monad_reader_lift (read)
 
 class monad_reader_functor (r r' : out_param (Type u)) (m : out_param (Type u → Type v)) (n n' : Type u → Type w) :=
 [functor {} : monad_functor_t (reader_t r m) (reader_t r' m) n n']
@@ -61,17 +63,8 @@ class monad_reader_functor (r r' : out_param (Type u)) (m : out_param (Type u �
 attribute [instance] monad_reader_functor.mk
 local attribute [instance] monad_reader_functor.functor
 
+def with_reader_t {r r' m} [monad m] {α} (f : r' → r) : reader_t r m α → reader_t r' m α :=
+λ x, ⟨λ r, x.run (f r)⟩
+
 def with_reader {r r'} {m n n'} [monad m] [monad_reader_functor r r' m n n'] {α : Type u} (f : r' → r) : n α → n' α :=
 monad_map $ λ α, (with_reader_t f : reader_t r m α → reader_t r' m α)
-
-def map_reader_t {r m m'} [monad m] [monad m'] {α} (f : Π {α}, m α → m' α) : reader_t r m α → reader_t r m' α :=
-λ x r, f (x r)
-
-instance (r m m') [monad m] [monad m'] : monad_functor m m' (reader_t r m) (reader_t r m') :=
-⟨@map_reader_t r m m' _ _⟩
-
-instance (r m) [monad m] : monad_reader r (reader_t r m) :=
-{ reader := λ α f, pure ∘ f }
-
-instance monad_reader_lift (r m m') [has_monad_lift m m'] [monad m] [monad_reader r m] [monad m'] : monad_reader r m' :=
-{ reader := λ α, monad_lift ∘ (monad_reader.reader : _ → m α) }
