leanpkg/leanpkg/main.lean
@@ -124,7 +124,7 @@ def fixup_git_version (dir : string) : ∀ (src : source), io source
 | src := return src
 
 def add (dep : dependency) : io unit := do
-(_, assg) ← materialize "." dep assignment.empty,
+(_, assg) ← (materialize "." dep).run assignment.empty,
 some downloaded_path ← return (assg.find dep.name),
 manif ← manifest.from_file (downloaded_path ++ "/" ++ leanpkg_toml_fn),
 src ← fixup_git_version downloaded_path dep.src,
