library/init/category/lawful.lean
@@ -76,59 +76,91 @@ lemma map_ext_congr {α β} {m : Type u → Type v} [has_map m] {x : m α} {f : 
 
 -- instances of previously defined monads
 
+namespace state_t
+section
+  variable  {σ : Type u}
+  variable  {m : Type u → Type v}
+  variable  [monad m]
+  variables {α β : Type u}
+  variables (x : state_t σ m α) (st : σ)
+
+  lemma ext {x x' : state_t σ m α} (h : ∀ st, x.run st = x'.run st) : x = x' :=
+  by cases_type* state_t; simp [show x = x', from funext h]
+
+  @[simp] lemma run_pure (a) : (pure a : state_t σ m α).run st = pure (a, st) := rfl
+  @[simp] lemma run_bind (f : α → state_t σ m β) : (x >>= f).run st = x.run st >>= λ p, (f p.1).run p.2 :=
+  by simp [bind, state_t.bind, state_t.run]; rw bind_ext_congr; intro a; cases a; simp [state_t.bind, state_t.run]
+  @[simp] lemma run_map (f : α → β) [is_lawful_monad m] : (f <$> x).run st = (λ p : α × σ, (f (prod.fst p), prod.snd p)) <$> x.run st :=
+  begin
+    rw ←bind_pure_comp_eq_map m,
+    change (x >>= pure ∘ f).run st = _,
+    simp
+  end
+end
+end state_t
+
 instance (m : Type u → Type v) [monad m] [is_lawful_monad m] (σ : Type u) : is_lawful_monad (state_t σ m) :=
-{ id_map := begin
-    intros, funext,
-    simp [(<$>), state_t.bind, state_t.return, function.comp, return],
-    rw [bind_ext_congr pure], swap,
-    { intros, cases a, refl },
-    { simp [bind_pure] }
-  end,
-  pure_bind := begin
-    intros, funext,
-    simp [bind, pure, has_pure.pure, state_t.bind, state_t.return, pure_bind],
-  end,
-  bind_assoc := begin
-    intros, funext,
-    simp [bind, state_t.bind, state_t.return, bind_assoc],
-    apply congr_arg, funext r,
-    cases r, refl
-  end }
+{ id_map := by intros; apply state_t.ext; intro; simp; erw id_map,
+  pure_bind := by intros; apply state_t.ext; intro; simp,
+  bind_assoc := by intros; apply state_t.ext; intro; simp [bind_assoc] }
 
 
-instance (ε : Type u) : is_lawful_monad (except ε) :=
-{ id_map := begin intros, cases x; refl, end,
-  pure_bind := begin intros; refl end,
-  bind_pure_comp_eq_map := begin intros, cases x; refl end,
-  bind_assoc := begin intros, cases x; reflexivity end }
+namespace except_t
+  variables {α β ε : Type u} {m : Type u → Type v} [monad m] (x : except_t ε m α)
 
-local attribute [simp] except_t.map except_t.bind except_t.return except_t.monad
+  lemma ext {x x' : except_t ε m α} (h : x.run = x'.run) : x = x' :=
+  by cases_type* except_t; simp * at *
+
+  @[simp] lemma run_pure (a) : (pure a : except_t ε m α).run = pure (@except.ok ε α a) := rfl
+  @[simp] lemma run_bind (f : α → except_t ε m β) : (x >>= f).run = x.run >>= except_t.bind_cont f := rfl
+  @[simp] lemma run_map (f : α → β) [is_lawful_monad m] : (f <$> x).run = except.map f <$> x.run :=
+  begin
+    rw ←bind_pure_comp_eq_map m,
+    change (x >>= pure ∘ f).run = _,
+    simp,
+    rw [bind_ext_congr],
+    intro a; cases a; simp [except_t.bind_cont, except.map]
+  end
+end except_t
 
 instance (m : Type u → Type v) [monad m] [is_lawful_monad m] (ε : Type u) : is_lawful_monad (except_t ε m) :=
 { id_map := begin
-    intros, cases x, dsimp,
-    rw map_ext_congr id; simp
+    intros, apply except_t.ext, simp,
+    rw [map_ext_congr, id_map],
+    intro a, cases a; refl
   end,
   bind_pure_comp_eq_map := begin
-    intros, cases x, dsimp,
+    intros, apply except_t.ext, simp,
     rw [bind_ext_congr, bind_pure_comp_eq_map],
-    intro a, cases a; dsimp [except.monad, except.map]; refl
+    intro a, cases a; refl
   end,
   bind_assoc := begin
-    intros, cases x, dsimp, simp [bind_assoc],
+    intros, apply except_t.ext, simp [bind_assoc],
     rw [bind_ext_congr],
-    { intro a, cases a; simp }
+    { intro a, cases a; simp [except_t.bind_cont] }
   end,
-  pure_bind := begin
-    intros, dsimp, simp,
-    cases f x, refl
-  end,
-  ..except_t.monad }
+  pure_bind := by intros; apply except_t.ext; simp [except_t.bind_cont] }
 
 
-local attribute [simp] reader_t.bind reader_t.pure
+namespace reader_t
+section
+  variable  {r : Type u}
+  variable  {m : Type u → Type v}
+  variable  [monad m]
+  variables {α β : Type u}
+  variables (x : reader_t r m α) (cfg : r)
+
+  lemma ext {x x' : reader_t r m α} (h : ∀ cfg, x.run cfg = x'.run cfg) : x = x' :=
+  by cases_type* reader_t; simp [show x = x', from funext h]
+
+  @[simp] lemma run_pure (a) : (pure a : reader_t r m α).run cfg = pure a := rfl
+  @[simp] lemma run_bind (f : α → reader_t r m β) : (x >>= f).run cfg = x.run cfg >>= λ a, (f a).run cfg := rfl
+  @[simp] lemma run_map (f : α → β) [is_lawful_monad m] : (f <$> x).run cfg = f <$> x.run cfg :=
+  by rw ←bind_pure_comp_eq_map m; refl
+end
+end reader_t
 
 instance (r : Type u) (m : Type u → Type v) [monad m] [is_lawful_monad m] : is_lawful_monad (reader_t r m) :=
-{ id_map := by intros; dsimp [reader_t.monad]; simp,
-  pure_bind := by intros; dsimp [reader_t.monad]; simp,
-  bind_assoc := by intros; dsimp [reader_t.monad]; simp [bind_assoc] }
+{ id_map := by intros; apply reader_t.ext; intro; simp,
+  pure_bind := by intros; apply reader_t.ext; intro; simp,
+  bind_assoc := by intros; apply reader_t.ext; intro; simp [bind_assoc] }
