tests/lean/run/1562.lean
@@ -7,7 +7,7 @@ meta constant smt2_state : Type
 state_t smt2_state tactic α
 
 meta instance tactic_to_smt2_m (α : Type) : has_coe (tactic α) (smt2_m α) :=
-⟨ fun tc, fun s, do res ← tc, return (res, s) ⟩
+⟨ fun tc, ⟨fun s, do res ← tc, return (res, s)⟩ ⟩
 
 meta def reflect_arith_formula : expr → smt2_m term
 | `(has_zero.zero) := smt2.builder.int_const <$> tactic.eval_expr int `(has_zero.zero int)
