tests/lean/run/my_tac_class.lean
@@ -1,14 +1,12 @@
 meta def mytac :=
 state_t nat tactic
 
-meta instance : monad mytac :=
-state_t.monad
-
-meta instance : monad_state nat mytac :=
-state_t.monad_state
-
-meta instance : has_monad_lift tactic mytac :=
-state_t.has_monad_lift _
+section
+local attribute [reducible] mytac
+meta instance : monad mytac := by apply_instance
+meta instance : monad_state_lift nat tactic mytac := by apply_instance
+meta instance : has_monad_lift tactic mytac := by apply_instance
+end
 
 meta instance (α : Type) : has_coe (tactic α) (mytac α) :=
 ⟨monad_lift⟩
@@ -19,7 +17,7 @@ meta def step {α : Type} (t : mytac α) : mytac unit :=
 t >> return ()
 
 meta def istep {α : Type} (line0 col0 line col : nat) (t : mytac α) : mytac unit :=
-λ v s, result.cases_on (@scope_trace _ line col (λ_, t v s))
+⟨λ v s, result.cases_on (@scope_trace _ line col (λ_, t.run v s))
   (λ ⟨a, v⟩ new_s, result.success ((), v) new_s)
   (λ opt_msg_thunk e new_s,
     match opt_msg_thunk with
@@ -27,10 +25,10 @@ meta def istep {α : Type} (line0 col0 line col : nat) (t : mytac α) : mytac un
       let msg := λ _ : unit, msg_thunk () ++ format.line ++ to_fmt "value: " ++ to_fmt v ++ format.line ++ to_fmt "state:" ++ format.line ++ new_s^.to_format in
           interaction_monad.result.exception (some msg) (some ⟨line, col⟩) new_s
     | none := interaction_monad.silent_fail new_s
-    end)
+    end)⟩
 
 meta def execute (tac : mytac unit) : tactic unit :=
-tac 0 >> return ()
+tac.run 0 >> return ()
 
 meta def save_info (p : pos) : mytac unit :=
 do v ← get,
