tests/lean/run/using_smt3.lean
@@ -6,10 +6,10 @@ by using_smt $ smt_tactic.intros >> get_local `x >>= (fun a, trace a)
 open tactic_result
 
 meta def fail_if_success {α : Type} (t : smt_tactic α) : smt_tactic unit :=
-λ ss ts, match t ss ts with
+⟨λ ss ts, match t.run ss ts with
 | success _ _     := failed ts
 | exception _ _ _ := success ((), ss) ts
-end
+end⟩
 
 def my_smt_config : smt_config :=
 { pre_cfg := { zeta := tt } }
